\includegraphics[height=1.25cm]{images/pictograms/FEM}
\includegraphics[height=1.25cm]{images/pictograms/benchmark}
\includegraphics[height=1.25cm]{images/pictograms/3d}

%%%%%%%%%%%%%%%%%%%%%%%%%%%%%%%%%%%%%%%%%%%%%%%%%%%%%%%%%%%%%%%%%%%%%%%%%%%%%%%%%%%%%%%%%%%%

\lstinputlisting[language=bash,basicstyle=\small]{python_codes/fieldstone_17/keywords.ascii}

\begin{center}
\inpython
{\small Code: \url{https://github.com/cedrict/fieldstone/tree/master/python_codes/fieldstone_17}}
\end{center}

\par\noindent\rule{\textwidth}{0.4pt}
%%%%%%%%%%%%%%%%%%%%%%%%%%%%%%%%%%%%%%%%%%%%%%%%%%%%%%%%%%%%%%%%


When using $Q_1 \times P_0$ elements, this benchmark fails 
 because of the Dirichlet b.c. on all 6 sides and all three components.
However, as we will see, it does work well with $Q_2 \times Q_1$ elements. 

This benchmark begins by postulating a polynomial solution to the 3D Stokes 
equation (see \textcite{dobo04} (2004)):
\begin{equation}
\vec{v}
=
\left(
\begin{array}{c}
x+x^2+xy+x^3y \\
y + xy + y^2 + x^2 y^2\\
-2z - 3xz - 3yz - 5x^2 yz
\end{array}
\right)
\label{eqburrr}
\end{equation}
and
\begin{equation}
p = xyz + x^3 y^3z - 5/32
\end{equation}
While it is then trivial to verify that this velocity field is divergence-free,  
the corresponding body force of the Stokes equation can be computed by 
inserting this solution into the momentum equation with a given viscosity $\eta$
(constant or position/velocity/strain rate dependent). 
The domain is a unit cube and velocity boundary conditions 
simply use Eq. (\ref{MMM-eqburrr}). 
Following \textcite{busa13} (2013), the viscosity
is given by the smoothly varying function
\begin{equation}
\eta = \exp(1 - \beta(x(1 - x) + y(1 - y) + z(1 - z)))
\end{equation}

One can easily show that the ratio of viscosities $\eta^\star$
in the system follows $\eta^\star=\exp(-3\beta/4)$ so that choosing $\beta=10$ yields
$\eta^\star\simeq 1808$ and $\beta=20$ yields $\eta^\star\simeq 3.269\times10^6$.


We start from the momentum conservation equation:
\[
-{\vec \nabla}p + {\vec \nabla}\cdot (2 \eta \dot{\bm \varepsilon(\vec\upnu)}) = {\vec f}
\]
The $x$-component of this equation writes
\begin{eqnarray}
f_x 
&=& -\frac{\partial p}{\partial x} 
+\frac{\partial}{\partial x} (2\eta \dot{\epsilon}_{xx})
+\frac{\partial}{\partial y} (2\eta \dot{\epsilon}_{xy})
+\frac{\partial}{\partial z} (2\eta \dot{\epsilon}_{xz}) \\
&=& 
-\frac{\partial p}{\partial x} 
+2\eta\frac{\partial}{\partial x} \dot{\epsilon}_{xx}
+2\eta\frac{\partial}{\partial y} \dot{\epsilon}_{xy}
+2\eta\frac{\partial}{\partial z} \dot{\epsilon}_{xz} 
+2\frac{\partial \eta}{\partial x} \dot{\epsilon}_{xx}
+2\frac{\partial \eta}{\partial y} \dot{\epsilon}_{xy}
+2\frac{\partial \eta}{\partial z} \dot{\epsilon}_{xz} 
\end{eqnarray}


Let us compute all the block separately:
\begin{eqnarray}
\dot{\epsilon}_{xx}&=& 1+2x+y+3x^2y  \nonumber\\
\dot{\epsilon}_{yy}&=& 1+x+2y+2x^2y \nonumber\\
\dot{\epsilon}_{zz}&=& -2-3x-3y-5x^2y \nonumber\\
2 \dot{\epsilon}_{xy}&=& (x+x^3)+(y+2xy^2) = x+y+2xy^2+x^3 \nonumber\\
2 \dot{\epsilon}_{xz}&=& (0)+(-3z-10xyz) = -3z -10xyz  \nonumber\\
2 \dot{\epsilon}_{yz}&=& (0) + (-3z-5x^2z) = -3z-5x^2z   \nonumber
\end{eqnarray}
In passing, one can verify that 
$
\dot{\epsilon}_{xx}
+\dot{\epsilon}_{yy}
+\dot{\epsilon}_{zz}=0
$.
We further have
\begin{eqnarray}
\frac{\partial}{\partial x} 2\dot{\epsilon}_{xx}&=& 2(2 +6xy) \nonumber\\ 
\frac{\partial}{\partial y} 2\dot{\epsilon}_{xy}&=&  1+4xy \nonumber\\
\frac{\partial}{\partial z} 2\dot{\epsilon}_{xz}&=& -3 -10xy   \nonumber\\ 
\frac{\partial}{\partial x} 2\dot{\epsilon}_{xy}&=& 1+2y^2+3x^2 \nonumber\\ 
\frac{\partial}{\partial y} 2\dot{\epsilon}_{yy}&=& 2( 2+2x^2 ) \nonumber\\ 
\frac{\partial}{\partial z} 2\dot{\epsilon}_{yz}&=& -3-5x^2   \nonumber\\
\frac{\partial}{\partial x} 2\dot{\epsilon}_{xz}&=& -10yz \nonumber\\ 
\frac{\partial}{\partial y} 2\dot{\epsilon}_{yz}&=& 0  \nonumber\\ 
\frac{\partial}{\partial z} 2\dot{\epsilon}_{zz}&=& 2( 0 ) \nonumber\\
\frac{\partial p}{\partial x} &=& yz+3x^2y^3z\\
\frac{\partial p}{\partial y} &=& xz +3x^3y^2z \\
\frac{\partial p}{\partial z} &=& xy+x^3y^3
\end{eqnarray}

%The viscosity is chosen to be 
%\[
%\mu(x,y,z) = \exp \left[ 1-\beta ( x(1-x)+y(1-y)+z(1-z) )   \right]
%\]
\paragraph{Pressure normalisation} Here again, because Dirichlet boundary conditions are prescribed on all sides the 
pressure is known up to an arbitrary constant. This constant can be determined by (arbitrarily) choosing 
to normalised the pressure field as follows:
\begin{equation}
\int_\Omega p \; d\Omega = 0 \label{constr1}
\end{equation}
This is a single constraint associated to a single Lagrange multiplier $\lambda$ and the global Stokes system takes the form 
\[
\left(
\begin{array}{ccc}
\K & \G & 0 \\
\G^T & 0 & {\cal C}\\
0 & {\cal C}^T & 0
\end{array}
\right)
\left(
\begin{array}{c}
V \\ P \\ \lambda
\end{array}
\right)
\]
In this particular case the constraint matrix ${\cal C}$ is a vector and it only acts on the pressure degrees of freedom because
of Eq.(\ref{constr1}). Its exact expression is as follows:
\[
\int_\Omega p \; d\Omega = \sum_e \int_{\Omega_e}  p \; d\Omega 
=\sum_e \int_{\Omega_e}  \sum_{i} N^p_i p_i \; d\Omega  
=\sum_e \sum_i \left( \int_{\Omega_e}  N^p_i \; d\Omega \right)  p_i 
=\sum_e {\cal C}_e \cdot {\bm p}_e
\] 
where ${\bm p}_e$ is the list of pressure dofs of element $e$. The elemental constraint vector contains the 
corresponding pressure basis functions integrated over the element. These elemental constraints are then 
assembled into the vector ${\cal C}$.

%-----------------------------
\subsubsection*{Constant viscosity}

Choosing $\beta=0$ yields a constant velocity $\eta(x,y,z) = \exp(1) \simeq 2.718$
(and greatly simplifies the right-hand side) so that 
\begin{eqnarray}
\frac{\partial }{\partial x} \eta(x,y,z) &=& 0 \\
\frac{\partial }{\partial y} \eta(x,y,z) &=& 0 \\
\frac{\partial }{\partial z} \eta(x,y,z) &=& 0
\end{eqnarray}
and 
\begin{eqnarray}
f_x 
&=& 
-\frac{\partial p}{\partial x} 
+2\eta\frac{\partial}{\partial x} \dot{\epsilon}_{xx}
+2\eta\frac{\partial}{\partial y} \dot{\epsilon}_{xy}
+2\eta\frac{\partial}{\partial z} \dot{\epsilon}_{xz} \nonumber\\
&=&
-(yz+3x^2y^3z)
+ 2(2 +6xy) + (1+4xy) + (-3 -10xy)   \nonumber\\
&=&
-(yz+3x^2y^3z)
+\eta(2+6xy ) \nonumber\\
f_y 
&=&  
-\frac{\partial p}{\partial y} 
+2\eta\frac{\partial}{\partial x} \dot{\epsilon}_{xy}
+2\eta\frac{\partial}{\partial y} \dot{\epsilon}_{yy}
+2\eta\frac{\partial}{\partial z} \dot{\epsilon}_{yz}  \nonumber\\
&=&
-(xz +3x^3y^2z)
+
\eta(1+2y^2+3x^2)
+\eta 2( 2+2x^2 )  
+\eta(-3-5x^2) \nonumber\\
&=&
-(xz +3x^3y^2z)
+ \eta ( 2 + 2x^2 +  2y^2)
\nonumber\\ 
f_z 
&=&
-\frac{\partial p}{\partial z} 
+2\eta\frac{\partial}{\partial x} \dot{\epsilon}_{xz}
+2\eta\frac{\partial}{\partial y} \dot{\epsilon}_{yz}
+2\eta\frac{\partial}{\partial z} \dot{\epsilon}_{zz}  \nonumber\\
&=&
-(xy+x^3y^3) 
+ \eta (-10yz) + 0 + 0 \nonumber\\
&=&
-(xy+x^3y^3) 
+\eta (-10yz) \nonumber
\end{eqnarray}
Finally
\begin{equation}
\vec{f} = 
-
\left(
\begin{array}{c}
yz+3x^2y^3z\\
xz +3x^3y^2z \\
xy+x^3y^3
\end{array}
\right)
+\eta
\left(
\begin{array}{c}
2+6xy  \\
2 + 2x^2 +  2y^2 \\
-10yz 
\end{array}
\right)
\end{equation}

\begin{remark}
There seems to be a sign problem with Eq.(26) in \cite{busa13}.
\end{remark}

\begin{center}
\includegraphics[width=5cm]{python_codes/fieldstone_17/results_isoviscous/u}
\includegraphics[width=5cm]{python_codes/fieldstone_17/results_isoviscous/v}
\includegraphics[width=5cm]{python_codes/fieldstone_17/results_isoviscous/w}\\
\includegraphics[width=5cm]{python_codes/fieldstone_17/results_isoviscous/pressure}
\includegraphics[width=5cm]{python_codes/fieldstone_17/results_isoviscous/sr}\\
{\captionfont Velocity, pressure and strain rate fields on a 6x6x6 grid.}
\end{center}

\begin{center}
\includegraphics[width=8cm]{python_codes/fieldstone_17/results_isoviscous/errors.pdf}
\includegraphics[width=8cm]{python_codes/fieldstone_17/results_isoviscous/errors_sr.pdf}
\end{center}
Since the strain rate is the spatial derivative of the velocity field we should 
find that it converges like $h^2$ as expected. However I am quite puzzled as to why the convergence 
of $\dot{\varepsilon}_{xx}$ is quadratic 
but at the same time almost 2 orders of magnitude higher than the other 5 components which in turn 
converge abnormally fast like $h^3$.

%-----------------------------
\subsubsection*{Variable viscosity}
The spatial derivatives of the viscosity are then given by
\begin{eqnarray}
\frac{\partial }{\partial x} \eta(x,y,z) &=& -(1-2x)\beta \eta(x,y,z) \nonumber\\
\frac{\partial }{\partial y} \eta(x,y,z) &=& -(1-2y)\beta \eta(x,y,z) \nonumber\\
\frac{\partial }{\partial z} \eta(x,y,z) &=& -(1-2z)\beta \eta(x,y,z) \nonumber
\end{eqnarray}
and the right-hand side by
\begin{eqnarray}
\vec{f} 
&=& 
-
\left(
\begin{array}{c}
yz+3x^2y^3z\\
xz +3x^3y^2z \\
xy+x^3y^3
\end{array}
\right)
+\eta
\left(
\begin{array}{c}
2+6xy  \\
2 + 2x^2 +  2y^2 \\
-10yz 
\end{array}
\right) 
-(1-2x)\beta \eta (x,y,z)
\left(
\begin{array}{c}
2\dot{\epsilon}_{xx} \\
2\dot{\epsilon}_{xy} \\
2\dot{\epsilon}_{xz} \\
\end{array}
\right) \\
&&
-(1-2y)\beta \eta (x,y,z)
\left(
\begin{array}{c}
2\dot{\epsilon}_{xy} \\
2\dot{\epsilon}_{yy} \\
2\dot{\epsilon}_{yz} \\
\end{array}
\right)
-(1-2z)\beta \eta (x,y,z)
\left(
\begin{array}{c}
2\dot{\epsilon}_{xz} \\
2\dot{\epsilon}_{yz} \\
2\dot{\epsilon}_{zz} \\
\end{array}
\right) \nonumber\\
&=& 
-
\left(
\begin{array}{c}
yz+3x^2y^3z\\
xz +3x^3y^2z \\
xy+x^3y^3
\end{array}
\right)
+\eta
\left(
\begin{array}{c}
2+6xy  \\
2 + 2x^2 +  2y^2 \\
-10yz 
\end{array}
\right) 
-
(1-2x)\beta \eta 
\left(
\begin{array}{c}
2+4x+2y+6x^2y \\
x+y+2xy^2+x^3 \\
-3z -10xyz 
\end{array}
\right) \nn \\
&&
-(1-2y)\beta \eta
\left(
\begin{array}{c}
x+y+2xy^2+x^3 \\
2+2x+4y+4x^2y \\
-3z-5x^2z \\
\end{array}
\right)
-(1-2z)\beta \eta
\left(
\begin{array}{c}
-3z -10xyz \\
-3z-5x^2z \\
-4-6x-6y-10x^2y
\end{array}
\right) \nonumber
\end{eqnarray}

Note that at $(x,y,z)=(0,0,0)$, $\eta=\exp(1)$, 
and at $(x,y,z)=(0.5,0.5,0.5)$, $\eta=\exp(1-3\beta/4)$
so that the maximum 
viscosity ratio is given by 
\[
\eta^\star = \frac{\exp(1-3\beta/4)}{\exp(1)} = \exp(-3\beta/4)
\]
By varying $\beta$ between 1 and 22 we can get up to 7 orders of magnitude viscosity difference.


\begin{center}
\includegraphics[width=7cm]{python_codes/fieldstone_17/results_beta5/errors.pdf}
\includegraphics[width=7cm]{python_codes/fieldstone_17/results_beta5/errors_sr.pdf}\\
{\captionfont Obtained for $\beta=5$}
\end{center}


\begin{center}
\includegraphics[width=7cm]{python_codes/fieldstone_17/results_beta10/errors.pdf}
\includegraphics[width=7cm]{python_codes/fieldstone_17/results_beta10/errors_sr.pdf}\\
{\captionfont Obtained for $\beta=10$}
\end{center}

We see that with increasing viscosity contrasts higher and higher resolutions are needed to 
attain the expected convergence rates for velocity and pressure. As for strain rate convergence, 
as puzzled as before ...



\begin{center}
\includegraphics[width=7cm]{python_codes/fieldstone_17/results_beta5/velocity}
\includegraphics[width=7cm]{python_codes/fieldstone_17/results_beta5/q}\\
\includegraphics[width=7cm]{python_codes/fieldstone_17/results_beta5/eta}
\includegraphics[width=7cm]{python_codes/fieldstone_17/results_beta5/sr}\\
{\captionfont Obtained for a 10x10x10 mesh and $\beta=5$}
\end{center}

















%\begin{center}
%\includegraphics[width=5cm]{python_codes/fieldstone_stokes_sphere_3D/grid}
%\includegraphics[width=5cm]{python_codes/fieldstone_stokes_sphere_3D/vel}
%\includegraphics[width=5cm]{python_codes/fieldstone_stokes_sphere_3D/press}\\
%\includegraphics[width=5cm]{python_codes/fieldstone_stokes_sphere_3D/press2}
%\includegraphics[width=5cm]{python_codes/fieldstone_stokes_sphere_3D/visc}
%\includegraphics[width=5cm]{python_codes/fieldstone_stokes_sphere_3D/dens}\\
%{\small resolution is 24x24x24}
%\end{center}

