\begin{flushright} {\tiny {\color{gray} basis\_q2\_3D.tex}} \end{flushright}
%~~~~~~~~~~~~~~~~~~~~~~~~~~~~~~~~~~~~~~~~~~~~~~~~~~~~~~~~~~~~~~~~~~~~~~~~~~~~~~~~~~~~~~~~~~~~~~~~~~

\begin{center}
\input{tikz/tikz_q2}
\end{center}
Note that the figure above depicts an element in $x,y,z$ space, not the reference
element in $r,s,t$ space which is centered around the origin.

\begin{eqnarray}
\bN_{1} &=& 0.5r(r-1)  \cdot 0.5s(s-1) \cdot 0.5t(t-1) \nn\\
\bN_{2} &=& (1-r^2)    \cdot 0.5s(s-1) \cdot 0.5t(t-1) \nn\\
\bN_{3} &=& 0.5r(r+1)  \cdot 0.5s(s-1) \cdot 0.5t(t-1) \nn\\
\bN_{4} &=&  0.5r(r-1) \cdot (1-s^2)   \cdot 0.5t(t-1) \nn\\
\bN_{5} &=&  (1-r^2)   \cdot (1-s^2)   \cdot 0.5t(t-1) \nn\\
\bN_{6} &=& 0.5r(r+1)  \cdot (1-s^2)   \cdot 0.5t(t-1) \nn\\
\bN_{7} &=&  0.5r(r-1) \cdot 0.5s(s+1) \cdot 0.5t(t-1) \nn\\
\bN_{8} &=&  (1-r^2)   \cdot 0.5s(s+1) \cdot 0.5t(t-1) \nn\\
\bN_{9} &=& 0.5r(r+1)  \cdot 0.5s(s+1) \cdot 0.5t(t-1) \nn\\
\bN_{10}&=&  0.5r(r-1) \cdot 0.5s(s-1) \cdot (1-t^2) \nn\\
\bN_{11}&=&  (1-r^2)   \cdot 0.5s(s-1) \cdot (1-t^2) \nn\\
\bN_{12}&=& 0.5r(r+1)  \cdot 0.5s(s-1) \cdot (1-t^2) \nn\\
\bN_{13}&=&  0.5r(r-1) \cdot (1-s^2)   \cdot (1-t^2) \nn\\
\bN_{14}&=&  (1-r^2)   \cdot (1-s^2)   \cdot (1-t^2) \nn\\
\bN_{15}&=& 0.5r(r+1)  \cdot (1-s^2)   \cdot (1-t^2) \nn\\
\bN_{16}&=&  0.5r(r-1) \cdot 0.5s(s+1) \cdot (1-t^2) \nn\\
\bN_{17}&=&  (1-r^2)   \cdot 0.5s(s+1) \cdot (1-t^2) \nn\\
\bN_{18}&=& 0.5r(r+1)  \cdot 0.5s(s+1) \cdot (1-t^2) \nn\\
\bN_{19}&=&  0.5r(r-1) \cdot 0.5s(s-1) \cdot 0.5t(t+1) \nn\\
\bN_{20}&=&  (1-r^2)   \cdot 0.5s(s-1) \cdot 0.5t(t+1) \nn\\
\bN_{21}&=& 0.5r(r+1)  \cdot 0.5s(s-1) \cdot 0.5t(t+1) \nn\\
\bN_{22}&=&  0.5r(r-1) \cdot (1-s^2)   \cdot 0.5t(t+1) \nn\\
\bN_{23}&=&  (1-r^2)   \cdot (1-s^2)   \cdot 0.5t(t+1) \nn\\
\bN_{24}&=& 0.5r(r+1)  \cdot (1-s^2)   \cdot 0.5t(t+1) \nn\\
\bN_{25}&=&  0.5r(r-1) \cdot 0.5s(s+1) \cdot 0.5t(t+1) \nn\\
\bN_{26}&=&  (1-r^2)   \cdot 0.5s(s+1) \cdot 0.5t(t+1) \nn\\
\bN_{27}&=& 0.5r(r+1)  \cdot 0.5s(s+1) \cdot 0.5t(t+1) \nn
\end{eqnarray}






