WORK in PROGRESS. DUH.

We start from the Poisson equation for the gravity potential:
\begin{equation}
\Delta U = 4\pi \rho {\cal G}
\end{equation}
As a consequence, inside a domain where $\rho=0$, the equation becomes $\Delta U=0$.

Let us assume that the spherical coordinates are appropriate for the problem at hand, and that 
the potential can be decomposed as follows:
\[
U(r,\theta,\phi) = U_r(r) U\bot(\theta,\phi)
\]
The full Laplacian operator in spherical coordinates is given 
by\footnote{\url{https://en.wikipedia.org/wiki/Laplace_operator}}:
\[
\Delta U 
= 
\underbrace{\frac{1}{r^2} \frac{\partial }{\partial r}\left(r^2 \frac{\partial U}{\partial r}\right)}_{\Delta_r}
+
\underbrace{
\frac{1}{r^2 \sin\theta} \frac{\partial }{\partial \theta} \left(\sin\theta \frac{\partial U}{\partial \theta} \right) 
+
\frac{1}{r^2 \sin^2\theta} \frac{\partial^2 U }{\partial \phi^2}
}_{\Delta_\bot}
\]
we then have:
\[
(\Delta_r + \Delta_\bot)(U_r U_\bot)=0
\]
i.e., 
\[
U_\bot \Delta_r U_r + U_r \Delta_\bot U_\bot=0
\]
Assuming $U_\bot=\sum_l\sum_m U_{lm}Y_{lm}$, knowing that spherical 
harmonics functions verify
\[
r^2 \Delta_\bot Y_l^m(\theta,\phi) = -l(l+1) Y_l^m (\theta,\phi)
\]
and assuming for now that the problem at hand is 1st degree (l=1), then 
\[
\Delta_\bot Y_l^m(\theta,\phi) = -\frac{2}{r^2} Y_l^m (\theta,\phi)
\]
and then
\[
\Delta_r U_r - U_r \frac{2}{r^2}=0
\]
make a link with my 2018 paper. 
\newpage

In spherical coordinates, the Laplacian is given by
\[
\Delta = 
\frac{1}{r^2} \frac{\partial }{\partial r} \left( r^2 \frac{\partial }{\partial r} \right)
+
\frac{1}{r^2 \sin^2 \theta} \frac{\partial}{\partial \theta} \left( \sin\theta \frac{\partial }{\partial \theta} \right)
+
\frac{1}{r^2 \sin^2 \theta} \frac{\partial^2}{\partial \phi^2}
\]
We wish to solve Laplace's equation $\Delta T(r,\theta,\phi)=0$ using the method 
of separation of variables:
\[
T(r,\theta,\phi) = R(r) \Theta(\theta) \Phi(\phi)
\]
We can insert this decomposition into the Laplace equation and multiply it by $r^2/R\Theta\Phi$ to obtain
\[
\frac{1}{R} \frac{d}{dr} \left( r^2 \frac{dR}{dr} \right) 
+ 
\frac{1}{\Theta} \frac{1}{\sin \theta} \frac{d}{d\theta} \left( \sin \theta \frac{d\Theta}{d\theta} \right)
+
\frac{1}{\Phi} \frac{1}{\sin^2 \theta} \frac{d^2\Phi}{d\phi^2}
=
0
\]
For reasons that will become clear later, the separation constant  is taken to be $-m^2$:
\begin{equation}
\frac{1}{\Phi} \frac{d^2\Phi}{d\phi^2} = -m^2
\label{eq:spha2}
\end{equation}
and 
\begin{equation}
-\frac{\sin\theta}{\Theta} \frac{d}{d\theta} \left( \sin \theta \frac{d\Theta}{d\theta} \right)
- \frac{\sin^2\theta}{R} \frac{d}{dr} \left( r^2 \frac{dR}{dr} \right) = -m^2
\label{eq:spha2}
\end{equation}
The first equation yields
\[
\Phi(\phi) = 
\left\{
\begin{array}{c}
e^{im\phi} \\ e^{-im\phi}
\end{array}
\right.
\qquad\qquad 
\text{for} \; m=0,1,2,3,...
\]
Note that $m$ must be an integer since $\phi$ is a periodic variable and $\Phi(\phi + 2\pi) = \Phi(\phi)$. 
In the case of $m=0$, the general solution is $\Phi(\phi) = a\phi + b$, but we must choose $a=0$ to
be consistent with $\Phi(\phi + 2\pi) = \Phi(\phi)$. Hence in the case of $m = 0$, only one solution is
allowed.

Equation \ref{eq:spha2} can now be recast in the following form:
\begin{equation}
 \frac{1}{R} \frac{d}{dr} \left( r^2 \frac{dR}{dr} \right) 
= 
-\frac{1}{\Theta}\frac{1}{\sin\theta} \frac{d}{d\theta} \left( \sin \theta \frac{d\Theta}{d\theta} \right) 
+\frac{m^2}{\sin^2\theta} = l(l+1) \label{eq:spha3}
\end{equation}
where the separation variable at this step is denoted by $l(l + 1)$ for reasons that will shortly
become clear.
The resulting radial equation is 
\[
\frac{1}{R} \frac{d}{dr} \left( r^2 \frac{dR}{dr} \right)  = l(l+1)
\]
or, 
\[
r^2 \frac{d^2R}{dr^2} + 2 r \frac{dR}{dr} - l(l+1)R =0
\]
The solution is of the form $R=r^s$. To determine the exponent $s$, 
we insert this solution back into the above ODE. The end result is
\[
s(s+1)=l(l+1) \qquad \Rightarrow \qquad s=l \; \text{or} \; s=-l-1
\]
or, 
\[
R(r) = 
\left\{
\begin{array}{c}
r^l \\ r^{-(l+1)}
\end{array}
\right.
\]
Eq. (\ref{eq:spha3}) also yields:
\[
\frac{1}{\sin\theta} \frac{d}{d\theta} \left( \sin\theta \frac{d\Theta}{d\theta} \right) 
+
\left[ l(l+1) - \frac{m^2}{\sin^2\theta} \right] \Theta = 0
\]
One can then carry out the following change of variables $x=\cos\theta$ and $y=\Theta(\theta)$ so that 
the above equation reduces to:
\[
(1-x^2) \frac{d^2 y}{d x^2} - 2x \frac{dy}{dx} + 
\left[ l(l+1)-\frac{m^2}{\sin^2\theta} \right] y =0
\]
This equation is the differential equation for associated Legendre 
polynomials\footnote{\url{https://en.wikipedia.org/wiki/Associated_Legendre_polynomials}}.
\index{Associated Legendre polynomials}
We then have
\[
y=P_l^m(x) \qquad \text{for} \; l=0,1,2,3,... \quad \text{and} \; m=-l,-l+1,...0,...l=1,l
\]
and 
\[
P_l^m(x)= \frac{(-1)^m}{2^l \; l!} (1-x^2)^{m/2}
\frac{d^{l+m}}{dx^{l+m}} (x^2-1)^l
\]
with $m \geq 0$ and $l\geq 0$.

In our case the differential equation for the associated Legendre polynomials, given above, depends
on $m^2$ and is therefore not sensitive to the sign of $m$.
Consequently, $P_l^m(x)$ and $P_l^{-m}(x)$ must be equivalent solutions and 
hence proportional to each other, and one can show that
\[
P_l^{-m}(\cos\theta) = (-1)^m\frac{(l-m)!}{(l+m)} P_l^m(\cos\theta)
\]
Combining all the results obtained above, we have found that the general solution to
Laplace’s equation is of the form
\begin{mdframed}[backgroundcolor=blue!5]
\[
T(r,\theta,\phi) = 
\left\{
\begin{array}{c}
r^l \\ r^{-(l+1)}
\end{array}
\right\}
P_l^m(\cos\theta) 
\left\{
\begin{array}{c}
e^{im\phi} \\ e^{-im\phi}
\end{array}
\right\}
\]
\end{mdframed}
where $l=0,1,2,3,...$ and $m=-l,-l+1,...,l-1,l$.

When solving the Laplace’s equation in spherical coordinates, it is traditional
to introduce the spherical harmonics, $Y_l^m(\theta,\phi)$:
\[
Y_l^m(\theta,\phi) = (-1)^m \sqrt{\frac{2l+1}{4\pi} \frac{(l-m)!}{(l+m)!}} P_l^m(\cos\theta) e^{im\phi}
\] 



